compiler/dsl/coq/ReflexBase.v
@@ -47,6 +47,9 @@ Definition num_eq (n1 n2 : num) : {n1 = n2} + {n1 <> n2}.
   decide equality; apply ascii_dec.
 Qed.
 
+Let FALSE : num := Num "000" "000".
+Let TRUE  : num := Num "001" "000".
+
 Definition str : Set :=
   list ascii.
 
